
1:
- 0
- error
- error
- error
- error
- error
- error
- error
- error
- error

2:
- error

3:
- error

4:
-  = 
- 0 = 0
- 1 = 1
- 2 = 2
- 3 = 3
- error
- 10 = 10
- 11 = 11
- error
- -1 = -1
- -2 = -2
- error

5:
- succ
- succ(0) = 1
- succ(1) = 2
- succ(2) = 3
- succ(3) = 4
- error
- succ(300) = 301
- succ(301) = 302
- error
- succ(-1) = 0
- succ(-2) = -1
- succ(-3) = -2
- error

6:
- pred
- pred(1) = 0
- pred(2) = 1
- pred(3) = 2
- pred(4) = 3
- error
- pred(1024) = 1023
- error
- pred(0) = -1
- pred(-1) = -2
- pred(-2) = -3
- error

7:
- sum
- sum(1, 2) = 3
- sum(2, 1) = 3
- sum(0, 1) = 1
- sum(2, 3) = 5
- sum(3, 5) = 8
- error

8:
- error
- sum(0, x0) = x0
- sum(0, x1) = x1
- sum(0, x2) = x2
- error
- sum(x0, 0) = x0
- sum(x1, 0) = x1
- sum(x2, 0) = x2
- error
- sum(x0, x1) = sum(x1, x0)
- error

9:
- prod
- prod(4, 2) = 8
- prod(3, 4) = 12
- prod(3, -2) = -6
- prod(x0, x1) = prod(x1, x0)
- prod(x0, 0) = 0
- prod(x0, 1) = x0
- error

10:
- div
- div(4, 2) = 2
- div(4, 3) = 1
- div(4, 4) = 1
- div(4, 5) = 0
- div(5, 2) = 2
- div(6, -2) = -3
- div(5, -3) = -1
- div(-5, 3) = -1
- div(-5, -3) = 1
- div(x0, 1) = x0
- error

11:
- eq
- eq(x0, x0) = K
- eq(0, -2) = False
- eq(0, -1) = False
- eq(0, 0) = K
- eq(0, 1) = False
- eq(0, 2) = False
- error
- eq(1, -1) = False
- eq(1, 0) = False
- eq(1, 1) = K
- eq(1, 2) = False
- eq(1, 3) = False
- error
- eq(2, 0) = False
- eq(2, 1) = False
- eq(2, 2) = K
- eq(2, 3) = False
- eq(2, 4) = False
- error
- eq(19, 20) = False
- eq(20, 20) = K
- eq(21, 20) = False
- error
- eq(-19, -20) = False
- eq(-20, -20) = K
- eq(-21, -20) = False
- error

12:
- lt
- lt(0, -1) = False
- lt(0, 0) = False
- lt(0, 1) = K
- lt(0, 2) = K
- error
- lt(1, 0) = False
- lt(1, 1) = False
- lt(1, 2) = K
- lt(1, 3) = K
- error
- lt(2, 1) = False
- lt(2, 2) = False
- lt(2, 3) = K
- lt(2, 4) = K
- error
- lt(19, 20) = K
- lt(20, 20) = False
- lt(21, 20) = False
- error
- lt(-19, -20) = False
- lt(-20, -20) = False
- lt(-21, -20) = K
- error

13:
- modulate
- modulate(0) = ?
- modulate(1) = ?
- modulate(-1) = ?
- modulate(2) = ?
- modulate(-2) = ?
- error
- modulate(16) = ?
- modulate(-16) = ?
- error
- modulate(255) = ?
- modulate(-255) = ?
- modulate(256) = ?
- modulate(-256) = ?
- error

14:
- demodulate
- demodulate(modulate(x0)) = x0
- modulate(demodulate(x0)) = x0

15:
- ?
- error
- ?
- error
- error
- error
- error
- error
- error

16:
- negate
- negate(0) = 0
- negate(1) = -1
- negate(-1) = 1
- negate(2) = -2
- negate(-2) = 2
- error

17:
- error
- succ(succ(0)) = 2
- succ(succ(succ(0))) = 3
- succ(pred(x0)) = x0
- pred(succ(x0)) = x0
- pred(sum(x0, 1)) = x0
- sum(sum(2, 3), 4) = 9
- sum(2, sum(3, 4)) = 9
- sum(prod(2, 3), 4) = 10
- prod(2, sum(3, 4)) = 14
- succ = sum(1)
- pred = sum(negate(1))
- error

18:
- S
- S(x0, x1, x2) = x0(x2, x1(x2))
- S(sum, succ, 1) = 3
- S(prod, sum(1), 6) = 42
- error

19:
- C
- C(x0, x1, x2) = x0(x2, x1)
- C(sum, 1, 2) = 3
- error

20:
- B
- B(x0, x1, x2) = x0(x1(x2))
- B(succ, pred, x0) = x0
- error

21:
- K
- K(x0, x1) = x0
- K(1, 5) = 1
- error
- K(K, succ(5)) = K
- K(succ(5), K) = 6
- error

22:
- False
- False(x0, x1) = x1
- False = S(K)

23:
- pow2
- pow2 = S(C(eq(0), 1), B(prod(2), B(pow2, sum(-1))))
- pow2(0) = S(C(eq(0), 1), B(prod(2), B(pow2, sum(-1))), 0)
- pow2(0) = C(eq(0), 1, 0, B(prod(2), B(pow2, sum(-1)), 0))
- pow2(0) = eq(0, 0, 1, B(prod(2), B(pow2, sum(-1)), 0))
- pow2(0) = K(1, B(prod(2), B(pow2, sum(-1)), 0))
- pow2(0) = 1
- pow2(1) = S(C(eq(0), 1), B(prod(2), B(pow2, sum(-1))), 1)
- pow2(1) = C(eq(0), 1, 1, B(prod(2), B(pow2, sum(-1)), 1))
- pow2(1) = eq(0, 1, 1, B(prod(2), B(pow2, sum(-1)), 1))
- pow2(1) = False(1, B(prod(2), B(pow2, sum(-1)), 1))
- pow2(1) = B(prod(2), B(pow2, sum(-1)), 1)
- pow2(1) = prod(2, B(pow2, sum(-1), 1))
- pow2(1) = prod(2, pow2(sum(-1, 1)))
- pow2(1) = prod(2, S(C(eq(0), 1), B(prod(2), B(pow2, sum(-1))), sum(-1, 1)))
- pow2(1) = prod(2, C(eq(0), 1, sum(-1, 1), B(prod(2), B(pow2, sum(-1)), sum(-1, 1))))
- pow2(1) = prod(2, eq(0, sum(-1, 1), 1, B(prod(2), B(pow2, sum(-1)), sum(-1, 1))))
- pow2(1) = prod(2, eq(0, 0, 1, B(prod(2), B(pow2, sum(-1)), sum(-1, 1))))
- pow2(1) = prod(2, K(1, B(prod(2), B(pow2, sum(-1)), sum(-1, 1))))
- pow2(1) = prod(2, 1)
- pow2(1) = 2
- pow2(2) = S(C(eq(0), 1), B(prod(2), B(pow2, sum(-1))), 2)
- error
- pow2(2) = 4
- pow2(3) = 8
- pow2(4) = 16
- pow2(5) = 32
- pow2(6) = 64
- pow2(7) = 128
- pow2(8) = 256
- error

24:
- error
- error
- error
- error
- error
- error
- error

25:
- Cons
- Cons(x0, x1, x2) = x2(x0, x1)

26:
- Car
- Car(Cons(x0, x1)) = x0
- Car(x2) = x2(K)

27:
- Cdr
- Cdr(Cons(x0, x1)) = x1
- Cdr(x2) = x2(False)

28:
- nil
- nil(x0) = K

29:
- isemptylist
- isemptylist(nil) = K
- isemptylist(Cons(x0, x1)) = False

30:
- [, ]
- [] = nil
- [x0] = Cons(x0, nil)
- [x0, x1] = Cons(x0, Cons(x1, nil))
- [x0, x1, x2] = Cons(x0, Cons(x1, Cons(x2, nil)))
- [x0, x1, x2, x5] = Cons(x0, Cons(x1, Cons(x2, Cons(x5, nil))))
- error

31:
- point
- point = Cons

32:
- draw
- draw([]) = ?
- draw([point(1, 1)]) = ?
- draw([point(1, 2)]) = ?
- draw([point(2, 5)]) = ?
- draw([point(1, 2), point(3, 1)]) = ?
- draw([point(5, 3), point(6, 3), point(4, 4), point(6, 4), point(4, 5)]) = ?
- error

33:
- ?
- error
- ?(7, 0) = ?
- ?(13, 0) = ?

34:
- ?
- ?(nil) = nil
- ?(Cons(x0, x1)) = Cons(draw(x0), ?(x1))

35:
- error
- modulate(nil) = ?
- modulate(Cons(nil, nil)) = ?
- modulate(Cons(0, nil)) = ?
- modulate(Cons(1, 2)) = ?
- modulate(Cons(1, Cons(2, nil))) = ?
- modulate([1, 2]) = ?
- modulate([1, [2, 3], 4]) = ?
- error

36:
- ?
- ?([0]) = [1, ?]

37:
- ?
- ?(0, x0, x1) = x0
- ?(1, x0, x1) = x1

38:
- ?
- ?(x0) = demodulate(modulate(x0))
- ?(x0) = ?(Car(x0), [?(Car(Cdr(x0))), ?(Car(Cdr(Cdr(x0))))], ?(?(Car(Cdr(x0))), ?(Car(Cdr(Cdr(x0))))))
- ?(x2, x4, x5) = ?(x2(x4, x5))

39:
- ?
- ?(x0, nil, point(0, 0)) = [x16, ?(x64)]
- ?(x0, x16, point(x1, x2)) = [x17, ?(x65)]
- ?(x0, x17, point(x3, x4)) = [x18, ?(x66)]
- ?(x0, x18, point(x5, x6)) = [x19, ?(x67)]
- error

40:
- ?(?)
- ?(x0, x1) = [0, nil, [[x1]]]
- ? = C(B(B, B(B(Cons(0)), C(B(B, Cons), C(Cons, nil)))), C(B(Cons, C(Cons, nil)), nil))
- ?(?, nil, point(1, 0)) = [nil, [?]]
- ?(?, nil, point(2, 3)) = [nil, [?]]
- ?(?, nil, point(4, 1)) = [nil, [?]]
- error

41:
- ?(?)
- ?(x0, x1) = [0, Cons(x1, x0), [Cons(x1, x0)]]
- ? = B(B(S(B(B(Cons(0)), C(B(B, Cons), C(Cons, nil))), C(Cons, nil))), C(Cons))
- ?(?, nil, point(0, 0)) = [[point(0, 0)], [?]]
- ?(?, [point(0, 0)], point(2, 3)) = [x2, [?]]
- ?(?, x2, point(1, 2)) = [x3, [?]]
- ?(?, x3, point(3, 2)) = [x4, [?]]
- ?(?, x4, point(4, 0)) = [x5, [?]]
- error

42:
- error

